VOQC/extraction/RotationMerging.ml
@@ -1,11 +1,14 @@
+open Datatypes
 open FMapAVL
+open FSetAVL
 open ListRepresentation
 open OrderedTypeEx
-open RzQGateSet
 
 type __ = Obj.t
 
-module FMap = Make(Nat_as_OT)
+module FSet = Make(Nat_as_OT)
+
+module FMap = FMapAVL.Make(Nat_as_OT)
 
 (** val xor : FSet.t -> FSet.t -> FSet.t **)
 
@@ -20,9 +23,11 @@ let get_set smap q =
   | None -> FSet.add q FSet.empty
 
 (** val find_merge' :
-    coq_RzQ_ucom_l -> FSet.t -> FSet.t -> FSet.elt -> FSet.t FMap.t -> int ->
-    coq_RzQ_Unitary gate_app list -> (((coq_RzQ_Unitary gate_app
-    list * Q.t) * int) * coq_RzQ_Unitary gate_list) option **)
+    RzQGateSet.coq_RzQ_ucom_l -> FSet.t -> FSet.t -> FSet.elt -> FSet.t
+    FMap.t -> int -> RzQGateSet.RzQGateSet.coq_RzQ_Unitary gate_app list ->
+    (((RzQGateSet.RzQGateSet.coq_RzQ_Unitary gate_app
+    list * Q.t) * int) * RzQGateSet.RzQGateSet.coq_RzQ_Unitary gate_list)
+    option **)
 
 let rec find_merge' l qs blst q smap n acc =
   (fun fO fS n -> if n=0 then fO () else fS (n-1))
@@ -30,41 +35,42 @@ let rec find_merge' l qs blst q smap n acc =
     (fun n' ->
     if FSet.equal qs blst
     then None
-    else (match next_gate l qs with
+    else (match next_gate l (fun q0 -> FSet.mem q0 qs) with
           | Some p ->
             let (p0, l2) = p in
             let (l1, g) = p0 in
             (match g with
              | App1 (r, q') ->
                (match r with
-                | URzQ_H ->
+                | RzQGateSet.RzQGateSet.URzQ_H ->
                   find_merge' l2 qs (FSet.add q' blst) q smap n'
-                    (List.append ((coq_H q') :: []) (List.rev_append l1 acc))
-                | URzQ_Rz a ->
+                    (List.append ((RzQGateSet.coq_H q') :: [])
+                      (List.rev_append l1 acc))
+                | RzQGateSet.RzQGateSet.URzQ_Rz a ->
                   let s = get_set smap q' in
                   let sorig = FSet.add q FSet.empty in
                   if (&&) (not (FSet.mem q' blst)) (FSet.equal s sorig)
                   then Some ((((List.rev_append acc l1), a), q'), l2)
                   else find_merge' l2 qs blst q smap n'
-                         (List.append ((coq_Rz a q') :: [])
+                         (List.append ((RzQGateSet.coq_Rz a q') :: [])
                            (List.rev_append l1 acc))
                 | _ -> None)
              | App2 (r, q1, q2) ->
                (match r with
-                | URzQ_CNOT ->
+                | RzQGateSet.RzQGateSet.URzQ_CNOT ->
                   let qs' = FSet.add q1 (FSet.add q2 qs) in
                   if (||) (FSet.mem q1 blst) (FSet.mem q2 blst)
                   then let blst' =
                          if FSet.mem q1 blst then FSet.add q2 blst else blst
                        in
                        find_merge' l2 qs' blst' q smap n'
-                         (List.append ((coq_CNOT q1 q2) :: [])
+                         (List.append ((RzQGateSet.coq_CNOT q1 q2) :: [])
                            (List.rev_append l1 acc))
                   else let s1 = get_set smap q1 in
                        let s2 = get_set smap q2 in
                        let smap' = FMap.add q2 (xor s1 s2) smap in
                        find_merge' l2 qs' blst q smap' n'
-                         (List.append ((coq_CNOT q1 q2) :: [])
+                         (List.append ((RzQGateSet.coq_CNOT q1 q2) :: [])
                            (List.rev_append l1 acc))
                 | _ -> None)
              | App3 (_, _, _, _) -> None)
@@ -72,15 +78,18 @@ let rec find_merge' l qs blst q smap n acc =
     n
 
 (** val find_merge :
-    coq_RzQ_ucom_l -> FSet.elt -> (((coq_RzQ_Unitary gate_app
-    list * Q.t) * int) * coq_RzQ_Unitary gate_list) option **)
+    RzQGateSet.coq_RzQ_ucom_l -> FSet.elt ->
+    (((RzQGateSet.RzQGateSet.coq_RzQ_Unitary gate_app
+    list * Q.t) * int) * RzQGateSet.RzQGateSet.coq_RzQ_Unitary gate_list)
+    option **)
 
 let find_merge l q =
   find_merge' l (FSet.add q FSet.empty) FSet.empty q FMap.empty
     (List.length l) []
 
 (** val merge_at_beginning :
-    coq_RzQ_ucom_l -> Q.t -> FSet.elt -> coq_RzQ_Unitary gate_app list option **)
+    RzQGateSet.coq_RzQ_ucom_l -> Q.t -> FSet.elt ->
+    RzQGateSet.RzQGateSet.coq_RzQ_Unitary gate_app list option **)
 
 let merge_at_beginning l a q =
   match find_merge l q with
@@ -88,11 +97,13 @@ let merge_at_beginning l a q =
     let (p0, l2) = p in
     let (p1, _) = p0 in
     let (l1, a') = p1 in
-    Some (List.append (combine_rotations a a' q) (List.append l1 l2))
+    Some
+    (List.append (RzQGateSet.combine_rotations a a' q) (List.append l1 l2))
   | None -> None
 
 (** val merge_at_end :
-    coq_RzQ_ucom_l -> Q.t -> FSet.elt -> coq_RzQ_Unitary gate_app list option **)
+    RzQGateSet.coq_RzQ_ucom_l -> Q.t -> FSet.elt ->
+    RzQGateSet.RzQGateSet.coq_RzQ_Unitary gate_app list option **)
 
 let merge_at_end l a q =
   match find_merge l q with
@@ -100,12 +111,13 @@ let merge_at_end l a q =
     let (p0, l2) = p in
     let (p1, q') = p0 in
     let (l1, a') = p1 in
-    Some (List.append l1 (List.append (combine_rotations a a' q') l2))
+    Some
+    (List.append l1 (List.append (RzQGateSet.combine_rotations a a' q') l2))
   | None -> None
 
 (** val merge_rotations_at_beginning :
-    coq_RzQ_ucom_l -> int -> coq_RzQ_Unitary gate_app list -> coq_RzQ_Unitary
-    gate_app list **)
+    RzQGateSet.coq_RzQ_ucom_l -> int -> RzQGateSet.RzQGateSet.coq_RzQ_Unitary
+    gate_app list -> RzQGateSet.RzQGateSet.coq_RzQ_Unitary gate_app list **)
 
 let rec merge_rotations_at_beginning l n acc =
   (fun fO fS n -> if n=0 then fO () else fS (n-1))
@@ -117,18 +129,19 @@ let rec merge_rotations_at_beginning l n acc =
       (match g with
        | App1 (r, q) ->
          (match r with
-          | URzQ_Rz a ->
+          | RzQGateSet.RzQGateSet.URzQ_Rz a ->
             (match merge_at_beginning t0 a q with
              | Some t' -> merge_rotations_at_beginning t' n' acc
              | None ->
-               merge_rotations_at_beginning t0 n' ((coq_Rz a q) :: acc))
+               merge_rotations_at_beginning t0 n'
+                 ((RzQGateSet.coq_Rz a q) :: acc))
           | _ -> merge_rotations_at_beginning t0 n' (g :: acc))
        | _ -> merge_rotations_at_beginning t0 n' (g :: acc)))
     n
 
 (** val merge_rotations_at_end :
-    coq_RzQ_ucom_l -> int -> coq_RzQ_Unitary gate_app list -> coq_RzQ_Unitary
-    gate_app list **)
+    RzQGateSet.coq_RzQ_ucom_l -> int -> RzQGateSet.RzQGateSet.coq_RzQ_Unitary
+    gate_app list -> RzQGateSet.RzQGateSet.coq_RzQ_Unitary gate_app list **)
 
 let rec merge_rotations_at_end l n acc =
   (fun fO fS n -> if n=0 then fO () else fS (n-1))
@@ -140,20 +153,24 @@ let rec merge_rotations_at_end l n acc =
       (match g with
        | App1 (r, q) ->
          (match r with
-          | URzQ_Rz a ->
+          | RzQGateSet.RzQGateSet.URzQ_Rz a ->
             (match merge_at_end t0 a q with
              | Some t' -> merge_rotations_at_end t' n' acc
-             | None -> merge_rotations_at_end t0 n' ((coq_Rz a q) :: acc))
+             | None ->
+               merge_rotations_at_end t0 n' ((RzQGateSet.coq_Rz a q) :: acc))
           | _ -> merge_rotations_at_end t0 n' (g :: acc))
        | _ -> merge_rotations_at_end t0 n' (g :: acc)))
     n
 
-(** val invert_gate : coq_RzQ_Unitary gate_app -> coq_RzQ_Unitary gate_app **)
+(** val invert_gate :
+    RzQGateSet.RzQGateSet.coq_RzQ_Unitary gate_app ->
+    RzQGateSet.RzQGateSet.coq_RzQ_Unitary gate_app **)
 
 let invert_gate g = match g with
-| App1 (y, q) -> (match y with
-                  | URzQ_Rz a -> invert_rotation a q
-                  | _ -> g)
+| App1 (r, q) ->
+  (match r with
+   | RzQGateSet.RzQGateSet.URzQ_Rz a -> RzQGateSet.invert_rotation a q
+   | _ -> g)
 | _ -> g
 
 (** val rev_append_w_map :
@@ -164,12 +181,16 @@ let rec rev_append_w_map f l l' =
   | [] -> l'
   | a :: l0 -> rev_append_w_map f l0 ((f a) :: l')
 
-(** val invert : coq_RzQ_ucom_l -> coq_RzQ_Unitary gate_app list **)
+(** val invert :
+    RzQGateSet.coq_RzQ_ucom_l -> RzQGateSet.RzQGateSet.coq_RzQ_Unitary
+    gate_app list **)
 
 let invert l =
   rev_append_w_map invert_gate l []
 
-(** val merge_rotations : coq_RzQ_ucom_l -> coq_RzQ_Unitary gate_app list **)
+(** val merge_rotations :
+    RzQGateSet.coq_RzQ_ucom_l -> RzQGateSet.RzQGateSet.coq_RzQ_Unitary
+    gate_app list **)
 
 let merge_rotations l =
   let l' = merge_rotations_at_beginning l (List.length l) [] in
