VOQC/extraction/RzQGateSet.ml
@@ -1,77 +1,99 @@
 open ListRepresentation
 
-type coq_RzQ_Unitary =
-| URzQ_H
-| URzQ_X
-| URzQ_Rz of Q.t
-| URzQ_CNOT
+module RzQGateSet =
+ struct
+  type coq_RzQ_Unitary =
+  | URzQ_H
+  | URzQ_X
+  | URzQ_Rz of Q.t
+  | URzQ_CNOT
 
-(** val coq_URzQ_T : coq_RzQ_Unitary **)
+  type coq_U = coq_RzQ_Unitary
 
-let coq_URzQ_T = URzQ_Rz (Q.of_ints 1 4)
+  (** val match_gate : int -> coq_U -> coq_U -> bool **)
 
-(** val coq_URzQ_P : coq_RzQ_Unitary **)
+  let match_gate _ u u' =
+    match u with
+    | URzQ_H -> (match u' with
+                 | URzQ_H -> true
+                 | _ -> false)
+    | URzQ_X -> (match u' with
+                 | URzQ_X -> true
+                 | _ -> false)
+    | URzQ_Rz q -> (match u' with
+                    | URzQ_Rz q' -> Q.equal q q'
+                    | _ -> false)
+    | URzQ_CNOT -> (match u' with
+                    | URzQ_CNOT -> true
+                    | _ -> false)
+ end
 
-let coq_URzQ_P = URzQ_Rz (Q.of_ints 1 2)
+(** val coq_URzQ_T : RzQGateSet.coq_RzQ_Unitary **)
 
-(** val coq_URzQ_Z : coq_RzQ_Unitary **)
+let coq_URzQ_T = RzQGateSet.URzQ_Rz (Q.of_ints 1 4)
 
-let coq_URzQ_Z = URzQ_Rz (Q.of_int 1)
+(** val coq_URzQ_P : RzQGateSet.coq_RzQ_Unitary **)
 
-(** val coq_URzQ_PDAG : coq_RzQ_Unitary **)
+let coq_URzQ_P = RzQGateSet.URzQ_Rz (Q.of_ints 1 2)
 
-let coq_URzQ_PDAG = URzQ_Rz (Q.of_ints 3 2)
+(** val coq_URzQ_Z : RzQGateSet.coq_RzQ_Unitary **)
 
-(** val coq_URzQ_TDAG : coq_RzQ_Unitary **)
+let coq_URzQ_Z = RzQGateSet.URzQ_Rz (Q.of_int 1)
 
-let coq_URzQ_TDAG = URzQ_Rz (Q.of_ints 7 4)
+(** val coq_URzQ_PDAG : RzQGateSet.coq_RzQ_Unitary **)
 
-(** val coq_T : int -> coq_RzQ_Unitary gate_app **)
+let coq_URzQ_PDAG = RzQGateSet.URzQ_Rz (Q.of_ints 3 2)
+
+(** val coq_URzQ_TDAG : RzQGateSet.coq_RzQ_Unitary **)
+
+let coq_URzQ_TDAG = RzQGateSet.URzQ_Rz (Q.of_ints 7 4)
+
+(** val coq_T : int -> RzQGateSet.coq_RzQ_Unitary gate_app **)
 
 let coq_T q =
   App1 (coq_URzQ_T, q)
 
-(** val coq_TDAG : int -> coq_RzQ_Unitary gate_app **)
+(** val coq_TDAG : int -> RzQGateSet.coq_RzQ_Unitary gate_app **)
 
 let coq_TDAG q =
   App1 (coq_URzQ_TDAG, q)
 
-(** val coq_P : int -> coq_RzQ_Unitary gate_app **)
+(** val coq_P : int -> RzQGateSet.coq_RzQ_Unitary gate_app **)
 
 let coq_P q =
   App1 (coq_URzQ_P, q)
 
-(** val coq_PDAG : int -> coq_RzQ_Unitary gate_app **)
+(** val coq_PDAG : int -> RzQGateSet.coq_RzQ_Unitary gate_app **)
 
 let coq_PDAG q =
   App1 (coq_URzQ_PDAG, q)
 
-(** val coq_Z : int -> coq_RzQ_Unitary gate_app **)
+(** val coq_Z : int -> RzQGateSet.coq_RzQ_Unitary gate_app **)
 
 let coq_Z q =
   App1 (coq_URzQ_Z, q)
 
-(** val coq_Rz : Q.t -> int -> coq_RzQ_Unitary gate_app **)
+(** val coq_Rz : Q.t -> int -> RzQGateSet.coq_RzQ_Unitary gate_app **)
 
 let coq_Rz i q =
-  App1 ((URzQ_Rz i), q)
+  App1 ((RzQGateSet.URzQ_Rz i), q)
 
-(** val coq_H : int -> coq_RzQ_Unitary gate_app **)
+(** val coq_H : int -> RzQGateSet.coq_RzQ_Unitary gate_app **)
 
 let coq_H q =
-  App1 (URzQ_H, q)
+  App1 (RzQGateSet.URzQ_H, q)
 
-(** val coq_X : int -> coq_RzQ_Unitary gate_app **)
+(** val coq_X : int -> RzQGateSet.coq_RzQ_Unitary gate_app **)
 
 let coq_X q =
-  App1 (URzQ_X, q)
+  App1 (RzQGateSet.URzQ_X, q)
 
-(** val coq_CNOT : int -> int -> coq_RzQ_Unitary gate_app **)
+(** val coq_CNOT : int -> int -> RzQGateSet.coq_RzQ_Unitary gate_app **)
 
 let coq_CNOT q1 q2 =
-  App2 (URzQ_CNOT, q1, q2)
+  App2 (RzQGateSet.URzQ_CNOT, q1, q2)
 
-type coq_RzQ_ucom_l = coq_RzQ_Unitary gate_list
+type coq_RzQ_ucom_l = RzQGateSet.coq_RzQ_Unitary gate_list
 
 (** val coq_CCX : int -> int -> int -> coq_RzQ_ucom_l **)
 
@@ -88,20 +110,19 @@ let coq_CCZ a b c =
     (coq_CNOT b c) :: ((coq_TDAG c) :: ((coq_CNOT a c) :: ((coq_CNOT a b) :: (
     (coq_TDAG b) :: ((coq_CNOT a b) :: ((coq_T a) :: ((coq_T b) :: ((coq_T c) :: []))))))))))))
 
-(** val match_gate : coq_RzQ_Unitary -> coq_RzQ_Unitary -> bool **)
+(** val remove_prefix :
+    coq_RzQ_ucom_l -> coq_RzQ_ucom_l -> RzQGateSet.coq_RzQ_Unitary gate_list
+    option **)
 
-let match_gate u u' =
-  match u with
-  | URzQ_H -> (match u' with
-               | URzQ_H -> true
-               | _ -> false)
-  | URzQ_X -> (match u' with
-               | URzQ_X -> true
-               | _ -> false)
-  | URzQ_Rz q -> (match u' with
-                  | URzQ_Rz q' -> Q.equal q q'
-                  | _ -> false)
-  | URzQ_CNOT -> false
+let remove_prefix l pfx =
+  remove_prefix l pfx RzQGateSet.match_gate
+
+(** val replace_pattern :
+    coq_RzQ_ucom_l -> coq_RzQ_ucom_l -> coq_RzQ_ucom_l ->
+    RzQGateSet.coq_RzQ_Unitary gate_list option **)
+
+let replace_pattern l pat rep =
+  replace_pattern l pat rep RzQGateSet.match_gate
 
 (** val bound : Q.t -> Q.t **)
 
@@ -121,7 +142,8 @@ let combine_rotations a a' q =
   let anew = bound (Q.add a a') in
   if Q.equal anew (Q.of_int 0) then [] else (coq_Rz anew q) :: []
 
-(** val invert_rotation : Q.t -> int -> coq_RzQ_Unitary gate_app **)
+(** val invert_rotation :
+    Q.t -> int -> RzQGateSet.coq_RzQ_Unitary gate_app **)
 
 let invert_rotation a q =
   coq_Rz (Q.sub (Q.of_int 2) a) q
