VOQC/src/optimizer/RzQGateSet.v
@@ -1,14 +1,12 @@
-Require Import UnitarySem.
-Require Import Equivalences.
 Require Export ListRepresentation.
-Require Import DensitySem.
-Require Import Setoid.
 Require Export QArith.
 
 Local Open Scope Z_scope.
 Local Open Scope Q_scope.
 
 (** RzQ Gate Set **)
+
+Module RzQGateSet <: GateSet.
 
 (* In our optimizer we use the gate set {H, X, RzQ, CNOT} where RzQ is
    rotation about the z-axis by i * PI / (2 ^ k) for integer i. We'll 
@@ -19,10 +17,41 @@ Inductive RzQ_Unitary : nat -> Set :=
   | URzQ_X           : RzQ_Unitary 1
   | URzQ_Rz (a : Q)  : RzQ_Unitary 1
   | URzQ_CNOT        : RzQ_Unitary 2.
+Definition U := RzQ_Unitary.
+
+Definition match_gate {n} (u u' : U n) : bool :=
+  match u, u' with
+  | URzQ_H, URzQ_H | URzQ_X, URzQ_X | URzQ_CNOT, URzQ_CNOT => true
+  | URzQ_Rz q, URzQ_Rz q' => Qeq_bool q q'
+  | _, _ => false
+  end.
+
+Definition to_base {n} (u : U n) :=
+  match u with
+  | URzQ_H     => U_R (PI/2) 0 PI
+  | URzQ_X     => U_R PI 0 PI
+  | URzQ_Rz a  => U_R 0 0 (Qreals.Q2R a * PI)%R
+  | URzQ_CNOT  => U_CNOT
+  end.
+
+Lemma match_gate_implies_eq : forall n (u u' : U n), 
+  match_gate u u' = true -> to_base u = to_base u'. 
+Proof.
+  intros n u u' H.
+  dependent destruction u; dependent destruction u'; 
+  auto; inversion H. simpl.
+  apply Qeq_bool_iff in H1.
+  apply f_equal. apply RMicromega.Q2R_m in H1. rewrite H1. reflexivity.
+Qed.
+
+End RzQGateSet.
+Export RzQGateSet.
+
+Module RzQProps := ListRepresentationProps RzQGateSet.
+Export RzQProps.
 
 (* Useful shorthands. *)
 
-(* Defining these constants makes extraction easier. *)
 Definition URzQ_I := URzQ_Rz 0.
 Definition URzQ_T := URzQ_Rz (1 / 4).
 Definition URzQ_P := URzQ_Rz (1 / 2).
@@ -42,7 +71,7 @@ Definition CNOT {dim} q1 q2 := @App2 _ dim URzQ_CNOT q1 q2.
 Definition RzQ_ucom dim := ucom RzQ_Unitary dim.
 Definition RzQ_ucom_l dim := gate_list RzQ_Unitary dim.
 Definition RzQ_com dim := com RzQ_Unitary dim.
-Definition RzQ_com_l dim := com_list RzQ_Unitary dim.
+(*Definition RzQ_com_l dim := com_list RzQ_Unitary dim.*)
 
 (* Used to convert benchmarks to PI4 set. *)
 Definition CCX {dim} a b c : RzQ_ucom_l dim :=
@@ -56,589 +85,13 @@ Definition CCZ {dim} a b c : RzQ_ucom_l dim :=
   CNOT a b :: TDAG b :: CNOT a b :: 
   T a :: T b :: T c :: []. 
 
-(* Conversion to the base gate set. *)
-Definition RzQ_to_base {n} (u : RzQ_Unitary n) : base_Unitary n :=
-  match u with
-  | URzQ_H     => U_R (PI/2) 0 PI
-  | URzQ_X     => U_R PI 0 PI
-  | URzQ_Rz a  => U_R 0 0 (Qreals.Q2R a * PI)%R
-  | URzQ_CNOT  => U_CNOT
-  end.
-
-Fixpoint RzQ_to_base_ucom_l {dim} (l : RzQ_ucom_l dim) : base_ucom_l dim :=
-  match l with
-  | [] => []
-  | (App1 u n) :: t => (App1 (RzQ_to_base u) n) :: (RzQ_to_base_ucom_l t)
-  | (App2 u m n) :: t => (App2 (RzQ_to_base u) m n) :: (RzQ_to_base_ucom_l t)
-  | _ => [] (* unreachable case *)
-  end.
-
-Fixpoint RzQ_to_base_instr {dim} (i : instr RzQ_Unitary dim) : instr base_Unitary dim :=
-  match i with
-  | UC u => UC (RzQ_to_base_ucom_l u)
-  | Meas n l1 l2 =>
-      let fix f l := match l with
-                     | [] => []
-                     | h :: t => (RzQ_to_base_instr h) :: (f t)
-                     end in
-      Meas n (f l1) (f l2)
-  end.
-Fixpoint RzQ_to_base_com_l {dim} (l : RzQ_com_l dim) : base_com_l dim :=
-  match l with
-  | [] => []
-  | h :: t => (RzQ_to_base_instr h) :: (RzQ_to_base_com_l t)
-  end.
-
-Lemma RzQ_to_base_instr_UC : forall dim (u : RzQ_ucom_l dim),
-  RzQ_to_base_instr (UC u) = UC (RzQ_to_base_ucom_l u).
-Proof. intros. reflexivity. Qed.
-
-Lemma RzQ_to_base_instr_Meas : forall dim n (l1 : RzQ_com_l dim) l2,
-  RzQ_to_base_instr (Meas n l1 l2) = Meas n (RzQ_to_base_com_l l1) (RzQ_to_base_com_l l2).
-Proof.
-  intros.
-  simpl.
-  apply f_equal2.
-  - induction l1; try rewrite IHl1; reflexivity.
-  - induction l2; try rewrite IHl2; reflexivity.
-Qed.
-Global Opaque RzQ_to_base_instr.
-
-Lemma RzQ_to_base_ucom_l_app : forall {dim} (l1 l2 : RzQ_ucom_l dim),
-  RzQ_to_base_ucom_l (l1 ++ l2) = (RzQ_to_base_ucom_l l1) ++ (RzQ_to_base_ucom_l l2).
-Proof.
-  intros.
-  induction l1.
-  - reflexivity.
-  - simpl; destruct a as [u | u | u]; dependent destruction u;
-    rewrite IHl1; reflexivity.
-Qed.    
-
-Lemma RzQ_to_base_ucom_l_WT : forall {dim} (l : RzQ_ucom_l dim), 
-  uc_well_typed_l l <-> uc_well_typed_l (RzQ_to_base_ucom_l l).
-Proof.
-  intros.
-  induction l; simpl.
-  - split; intros H; inversion H; constructor; assumption.
-  - destruct a as [u | u | u]; dependent destruction u;
-    split; intros H;
-    inversion H; subst;
-    constructor; try apply IHl; assumption.
-Qed.
-
-Lemma RzQ_to_base_com_l_app : forall {dim} (l1 l2 : RzQ_com_l dim),
-  RzQ_to_base_com_l (l1 ++ l2) = (RzQ_to_base_com_l l1) ++ (RzQ_to_base_com_l l2).
-Proof.
-  intros.
-  induction l1.
-  - reflexivity.
-  - simpl; rewrite IHl1; reflexivity.
-Qed. 
-
-Definition RzQ_eval {dim} (l : RzQ_ucom_l dim) :=
-  uc_eval (list_to_ucom (RzQ_to_base_ucom_l l)).
-
-(** Equivalence over RzQ_ucom_l. **)
-
-Local Open Scope ucom_scope.
-Definition uc_equiv_l {dim} (l1 l2 : RzQ_ucom_l dim) := 
-  (list_to_ucom (RzQ_to_base_ucom_l l1)) ≡ (list_to_ucom (RzQ_to_base_ucom_l l2)).
-Infix "=l=" := uc_equiv_l (at level 70) : ucom_scope.
-
-Lemma uc_equiv_l_refl : forall {dim} (l1 : RzQ_ucom_l dim), l1 =l= l1.
-Proof. easy. Qed.
- 
-Lemma uc_equiv_l_sym : forall {dim} (l1 l2 : RzQ_ucom_l dim), l1 =l= l2 -> l2 =l= l1.
-Proof. easy. Qed.
- 
-Lemma uc_equiv_l_trans : forall {dim} (l1 l2 l3 : RzQ_ucom_l dim), 
-  l1 =l= l2 -> l2 =l= l3 -> l1 =l= l3.
-Proof. intros dim l1 l2 l3 H12 H23. unfold uc_equiv_l in *. rewrite H12. easy. Qed.
-
-Lemma uc_cons_congruence : forall {dim} (g : gate_app RzQ_Unitary dim)  (l l' : RzQ_ucom_l dim),
-  l =l= l' ->
-  g :: l =l= g :: l'.
-Proof.
-  intros dim g l l' Hl.
-  unfold uc_equiv_l, uc_equiv.
-  simpl.
-  destruct g; simpl; try rewrite Hl; reflexivity.
-Qed.
-
-Lemma uc_app_congruence : forall {dim} (l1 l1' l2 l2' : RzQ_ucom_l dim),
-  l1 =l= l1' ->
-  l2 =l= l2' ->
-  l1 ++ l2 =l= l1' ++ l2'.
-Proof.
-  intros dim l1 l1' l2 l2' Hl1 Hl2.
-  unfold uc_equiv_l, uc_equiv.
-  simpl.
-  repeat rewrite RzQ_to_base_ucom_l_app, list_to_ucom_append; simpl.
-  rewrite Hl1, Hl2.
-  reflexivity.
-Qed.
-
-Add Parametric Relation (dim : nat) : (RzQ_ucom_l dim) (@uc_equiv_l dim)
-  reflexivity proved by uc_equiv_l_refl
-  symmetry proved by uc_equiv_l_sym
-  transitivity proved by uc_equiv_l_trans
-  as uc_equiv_l_rel.
-
-Add Parametric Morphism (dim : nat) : (@List.cons (gate_app RzQ_Unitary dim))
-  with signature eq ==> (@uc_equiv_l dim) ==> (@uc_equiv_l dim) as uc_cons_mor.
-Proof. intros y x0 y0 H0. apply uc_cons_congruence; easy. Qed.
-
-Add Parametric Morphism (dim : nat) : (@app (gate_app RzQ_Unitary dim))
-  with signature (@uc_equiv_l dim) ==> (@uc_equiv_l dim) ==> (@uc_equiv_l dim) as uc_app_mor.
-Proof. intros x y H x0 y0 H0. apply uc_app_congruence; easy. Qed.
-
-(* Useful relationship between equivalence and well-typedness. *)
-
-Lemma uc_equiv_l_implies_WT : forall {dim} (l l' : RzQ_ucom_l dim),
-  l =l= l' ->
-  uc_well_typed_l l ->
-  uc_well_typed_l l'.
-Proof.
-  intros dim l l' H WT.
-  apply RzQ_to_base_ucom_l_WT.
-  apply list_to_ucom_WT. 
-  apply uc_eval_nonzero_iff.
-  apply RzQ_to_base_ucom_l_WT in WT.
-  apply list_to_ucom_WT in WT.
-  apply uc_eval_nonzero_iff in WT.
-  rewrite <- H; assumption.
-Qed.
-
-(** Commutativity lemmas **)
-
-Lemma does_not_reference_commutes_app1 : forall {dim} (l : RzQ_ucom_l dim) u q,
-  does_not_reference l q = true ->
-  [App1 u q] ++ l =l= l ++ [App1 u q]. 
-Proof.
-  intros dim l u q H.
-  induction l.
-  - reflexivity.
-  - simpl in *.
-    destruct a as [u' | u' | u']; dependent destruction u';
-    apply andb_prop in H0 as [H1 H2];
-    repeat match goal with 
-    | H : does_not_reference_appl _ _ = true |- _ => apply negb_true_iff in H
-    end;
-    repeat match goal with 
-    | H : (_ || _) = false |- _ => apply orb_false_elim in H as [? ?]
-    end;
-    repeat match goal with
-    | H : (_ =? _)%nat = false |- _ => 
-         apply beq_nat_false in H;
-         apply not_eq_sym in H
-    end;
-    rewrite <- IHl; try assumption;
-    unfold uc_equiv_l; simpl; dependent destruction u; simpl;
-    rewrite <- 2 useq_assoc;
-    try rewrite U_V_comm;
-    try rewrite (U_CNOT_comm _ n n0);
-    try reflexivity;
-    try assumption.
-Qed.
-
-Lemma does_not_reference_commutes_app2 : forall {dim} (l : RzQ_ucom_l dim) u m n,
-  does_not_reference l m = true ->
-  does_not_reference l n = true ->
-  [App2 u m n] ++ l =l= l ++ [App2 u m n]. 
-Proof.
-  intros.
-  induction l.
-  - reflexivity.
-  - simpl in *.
-    destruct a as [u' | u' | u']; dependent destruction u';
-    apply andb_prop in H0 as [? ?];
-    apply andb_prop in H1 as [? ?];
-    repeat match goal with 
-    | H : does_not_reference_appl _ _ = true |- _ => apply negb_true_iff in H
-    end;
-    repeat match goal with 
-    | H : (_ || _) = false |- _ => apply orb_false_elim in H as [? ?]
-    end;
-    repeat match goal with
-    | H : (_ =? _)%nat = false |- _ => apply beq_nat_false in H    
-    end;
-    rewrite <- IHl; try assumption;
-    unfold uc_equiv_l; simpl; dependent destruction u; simpl;
-    rewrite <- 2 useq_assoc;
-    try rewrite (U_CNOT_comm n0 m n);
-    try rewrite (CNOT_CNOT_comm m n n0 n1);
-    try reflexivity;
-    assumption.
-Qed.
-
-Lemma nsqg_commutes : forall {dim} (l : RzQ_ucom_l dim) q u l1 l2,
-  next_single_qubit_gate l q = Some (l1, u, l2) -> 
-  l =l= [App1 u q] ++ l1 ++ l2.
-Proof.
-  intros dim l q u l1 l2 H.
-  specialize (nsqg_preserves_structure _ _ _ _ _ H) as H1.
-  subst.
-  apply nsqg_l1_does_not_reference in H.
-  apply (does_not_reference_commutes_app1 _ u _) in H.
-  repeat rewrite app_assoc.  
-  rewrite H.
-  reflexivity.
-Qed.
-
-Lemma lsqg_commutes : forall {dim} (l : RzQ_ucom_l dim) q u l1 l2,
-  last_single_qubit_gate l q = Some (l1, u, l2) -> 
-  l =l= l1 ++ l2 ++ [App1 u q].
-Proof.
-  intros dim l q u l1 l2 H.
-  specialize (lsqg_preserves_structure _ _ _ _ _ H) as H1.
-  subst.
-  apply lsqg_l2_does_not_reference in H.
-  apply (does_not_reference_commutes_app1 _ u _) in H.
-  rewrite H.
-  reflexivity.
-Qed.
-
-(** Equivalence up to a phase over RzQ_ucom_l. **)
-
-Definition uc_cong_l {dim} (l1 l2 : RzQ_ucom_l dim) := 
-  (list_to_ucom (RzQ_to_base_ucom_l l1)) ≅ (list_to_ucom (RzQ_to_base_ucom_l l2)).
-Infix "≅l≅" := uc_cong_l (at level 20).
-
-Lemma uc_cong_l_refl : forall {dim : nat} (l1 : RzQ_ucom_l dim), l1 ≅l≅ l1.
-Proof. intros. exists 0%R. rewrite Cexp_0. rewrite Mscale_1_l. reflexivity. Qed.
-
-Lemma uc_cong_l_sym : forall {dim : nat} (l1 l2 : RzQ_ucom_l dim), l1 ≅l≅ l2 -> l2 ≅l≅ l1.
-Proof. intros dim l1 l2 H. unfold uc_cong_l in *. rewrite H. reflexivity. Qed.
-
-Lemma uc_cong_l_trans : forall {dim : nat} (l1 l2 l3 : RzQ_ucom_l dim), l1 ≅l≅ l2 -> l2 ≅l≅ l3 -> l1 ≅l≅ l3.
-Proof.
-  intros dim l1 l2 l3 H1 H2.
-  unfold uc_cong_l in *.
-  eapply uc_cong_trans. apply H1. apply H2.
-Qed.  
-
-Lemma uc_cong_l_cons_congruence : forall {dim : nat} (g : gate_app RzQ_Unitary dim) (l l' : RzQ_ucom_l dim),
-  l ≅l≅ l' -> (g :: l) ≅l≅ (g :: l').
-Proof.
-  intros dim g l l' H. unfold uc_cong_l in *.
-  simpl.
-  inversion H.
-  destruct g as [u | u | u]; dependent destruction u;
-  exists x; simpl; rewrite <- Mscale_mult_dist_l; rewrite H1; reflexivity.
-Qed.
-
-Lemma uc_cong_l_app_congruence : forall {dim : nat} (l l' m m': RzQ_ucom_l dim),
-  l ≅l≅ l' -> m ≅l≅ m' -> (m ++ l) ≅l≅ (m' ++ l').
-Proof.
-  intros dim l l' m m' H1 H2.
-  unfold uc_cong_l in *.
-  inversion H1. inversion H2.
-  exists (x + x0)%R.
-  repeat rewrite RzQ_to_base_ucom_l_app, list_to_ucom_append; simpl.
-  rewrite H0. rewrite H3. 
-  rewrite Mscale_mult_dist_r.
-  rewrite Mscale_mult_dist_l.
-  rewrite Mscale_assoc.
-  rewrite <- Cexp_add.
-  rewrite Rplus_comm.
-  reflexivity.
-Qed.
-    
-Add Parametric Relation (dim : nat) : (RzQ_ucom_l dim) (@uc_cong_l dim)
-  reflexivity proved by uc_cong_l_refl
-  symmetry proved by uc_cong_l_sym
-  transitivity proved by uc_cong_l_trans
-  as uc_cong_l_rel.
-
-Add Parametric Morphism (dim : nat) : (@List.cons (gate_app RzQ_Unitary dim))
-  with signature eq ==> (@uc_cong_l dim) ==> (@uc_cong_l dim) as uc_cons_mor_cong.
-Proof. intros. apply uc_cong_l_cons_congruence. easy. Qed.
-
-Add Parametric Morphism (dim : nat) : (@app (gate_app RzQ_Unitary dim))
-  with signature (@uc_cong_l dim) ==> (@uc_cong_l dim) ==> (@uc_cong_l dim) as uc_app_mor_cong.
-Proof. intros x y H x0 y0 H0. apply uc_cong_l_app_congruence; easy. Qed.
-
-Lemma uc_equiv_cong_l : forall {dim : nat} (c c' : RzQ_ucom_l dim), c =l= c' -> c ≅l≅ c'.
-Proof.
-  intros dim c c' H.
-  exists 0%R. rewrite Cexp_0, Mscale_1_l. 
-  apply H.
-Qed.
-
-Lemma uc_cong_l_implies_WT : forall {dim} (l l' : RzQ_ucom_l dim),
-  l ≅l≅ l' ->
-  uc_well_typed_l l ->
-  uc_well_typed_l l'.
-Proof.
-  intros dim l l' H WT.
-  apply RzQ_to_base_ucom_l_WT.
-  apply list_to_ucom_WT. 
-  apply uc_eval_nonzero_iff.
-  apply RzQ_to_base_ucom_l_WT in WT.
-  apply list_to_ucom_WT in WT.
-  apply uc_eval_nonzero_iff in WT.
-  destruct H.
-  rewrite H0 in WT. 
-  intros contra.
-  rewrite contra in WT.
-  contradict WT.
-  Msimpl.
-  reflexivity.
-Qed.
-
-(* Soundness of replace_single_qubit_pattern. *)
-
-Definition match_gate (u u' : RzQ_Unitary 1) : bool :=
-  match u, u' with
-  | URzQ_H, URzQ_H | URzQ_X, URzQ_X => true
-  | URzQ_Rz q, URzQ_Rz q' => Qeq_bool q q'
-  | _, _ => false
-  end.
-
-Lemma match_gate_refl : forall (u u' : RzQ_Unitary 1), 
-  match_gate u u' = true -> RzQ_to_base u = RzQ_to_base u'. 
-Proof.
-  intros u u' H.
-  dependent destruction u; dependent destruction u';
-  inversion H0; try reflexivity.
-  simpl. apply Qeq_bool_eq in H2. rewrite H2. reflexivity.
-Qed.
-
-Lemma remove_single_qubit_pattern_correct : forall {dim} (l l' : RzQ_ucom_l dim) (q : nat) (pat : single_qubit_pattern RzQ_Unitary),
-  remove_single_qubit_pattern l q pat match_gate = Some l' ->
-  l =l= (single_qubit_pattern_to_program dim pat q) ++ l'.
-Proof.
-  intros.
-  generalize dependent l'.
-  generalize dependent l.
-  induction pat; intros l l' H.
-  - inversion H; subst. reflexivity.
-  - simpl in H. 
-    destruct (next_single_qubit_gate l q) eqn:nsqg; try discriminate.
-    repeat destruct p.
-    destruct (match_gate a r) eqn:Hmatch; try discriminate.
-    simpl.
-    rewrite <- (IHpat _ _ H). 
-    rewrite (nsqg_commutes _ _ _ _ _ nsqg).
-    apply match_gate_refl in Hmatch.
-    unfold uc_equiv_l; simpl.
-    rewrite Hmatch; reflexivity.
-Qed.
-
-(* Equivalence up to a phase. Exact equivalence is also easy to prove, but not used 
-   in our development. *)
-Lemma replace_single_qubit_pattern_sound : forall {dim} (l l' : RzQ_ucom_l dim) (q : nat) (pat rep : single_qubit_pattern RzQ_Unitary),
-  single_qubit_pattern_to_program dim pat q ≅l≅ single_qubit_pattern_to_program dim rep q ->
-  replace_single_qubit_pattern l q pat rep match_gate = Some l' ->
-  l ≅l≅ l'.
-Proof.
-  intros dim l l' q pat rep H1 H2.
-  unfold replace_single_qubit_pattern in H2.
-  destruct (remove_single_qubit_pattern l q pat) eqn:rem; try discriminate.
-  apply remove_single_qubit_pattern_correct in rem.
-  apply uc_equiv_cong_l in rem.
-  inversion H2; subst.
-  rewrite rem, H1. 
-  reflexivity.
-Qed.
-
-(** Equivalence over RzQ_com_l. **)
-
-Local Close Scope ucom_scope.
-Local Open Scope com_scope.
-Definition c_equiv_l {dim} (l1 l2 : RzQ_com_l dim) := 
-  (list_to_com (RzQ_to_base_com_l l1)) ≡ (list_to_com (RzQ_to_base_com_l l2)).
-Infix "=l=" := c_equiv_l (at level 70) : com_scope.
-
-Lemma c_equiv_l_refl : forall {dim} (l1 : RzQ_com_l dim), l1 =l= l1.
-Proof. easy. Qed.
- 
-Lemma c_equiv_l_sym : forall {dim} (l1 l2 : RzQ_com_l dim), l1 =l= l2 -> l2 =l= l1.
-Proof. unfold c_equiv_l. easy. Qed.
- 
-Lemma c_equiv_l_trans : forall {dim} (l1 l2 l3 : RzQ_com_l dim), 
-  l1 =l= l2 -> l2 =l= l3 -> l1 =l= l3.
-Proof. unfold c_equiv_l. intros dim l1 l2 l3 H12 H23. rewrite H12. easy. Qed.
-
-Lemma c_cons_congruence : forall {dim} (i : instr RzQ_Unitary dim)  (l l' : RzQ_com_l dim),
-  l =l= l' ->
-  i :: l =l= i :: l'.
-Proof.
-  unfold c_equiv_l.
-  intros dim i l l' Hl.  
-  simpl. rewrite Hl. reflexivity.
-Qed.
-
-Lemma c_app_congruence : forall {dim} (l1 l1' l2 l2' : RzQ_com_l dim),
-  l1 =l= l1' ->
-  l2 =l= l2' ->
-  l1 ++ l2 =l= l1' ++ l2'.
-Proof.
-  unfold c_equiv_l.
-  intros dim l1 l1' l2 l2' Hl1 Hl2.
-  repeat rewrite RzQ_to_base_com_l_app, list_to_com_append; simpl.
-  rewrite Hl1, Hl2.
-  reflexivity.
-Qed.
-
-Add Parametric Relation (dim : nat) : (RzQ_com_l dim) (@c_equiv_l dim)
-  reflexivity proved by c_equiv_l_refl
-  symmetry proved by c_equiv_l_sym
-  transitivity proved by c_equiv_l_trans
-  as c_equiv_l_rel.
-
-Add Parametric Morphism (dim : nat) : (@List.cons (instr RzQ_Unitary dim))
-  with signature eq ==> (@c_equiv_l dim) ==> (@c_equiv_l dim) as c_cons_mor.
-Proof. intros y x0 y0 H0. apply c_cons_congruence; easy. Qed.
-
-Add Parametric Morphism (dim : nat) : (@app (gate_app RzQ_Unitary dim))
-  with signature (@uc_equiv_l dim) ==> (@uc_equiv_l dim) ==> (@uc_equiv_l dim) as c_app_mor.
-Proof. intros x y H x0 y0 H0. apply uc_app_congruence; easy. Qed.
-
-(* Also useful to have a congruence lemma for rewriting inside Meas. *)
-Definition c_eval_l {dim} (l : RzQ_com_l dim) :=
-  c_eval (list_to_com (RzQ_to_base_com_l l)).
-Local Coercion Nat.b2n : bool >-> nat.
-Definition project_onto {dim} ρ n (b : bool) := super (@pad 1 n dim (∣b⟩ × ∣b⟩†)) ρ.
-Lemma Meas_cons_congruence : forall dim n (l1 l2 l1' l2' l l' : RzQ_com_l dim),
-  (forall ρ, WF_Matrix ρ ->
-   c_eval_l l1 (project_onto ρ n true) = c_eval_l l1' (project_onto ρ n true)) ->
-  (forall ρ, WF_Matrix ρ ->
-   c_eval_l l2 (project_onto ρ n false) = c_eval_l l2' (project_onto ρ n false)) ->
-  l =l= l' ->
-  Meas n l1 l2 :: l =l= Meas n l1' l2' :: l'.
-Proof.
-  intros.
-  unfold c_equiv_l; simpl.
-  repeat rewrite RzQ_to_base_instr_Meas, instr_to_com_Meas.
-  apply seq_congruence; auto.
-  unfold c_equiv; simpl.
-  intros Hdim ρ WFρ.
-  unfold Splus, compose_super; simpl.
-  unfold c_eval_l, project_onto in *.
-  simpl in *.
-  rewrite H0, H1; try assumption.
-  reflexivity.
-Qed.
-
-(** Commutativity lemmas for com list representation. **)
-
-Lemma uc_equiv_l_implies_c_equiv_l : forall dim (u u' : RzQ_ucom_l dim),
-  (u =l= u')%ucom ->
-  [UC u] =l= [UC u'].
-Proof.
-  unfold uc_equiv_l, uc_equiv, c_equiv_l, c_equiv.
-  intros dim u u' H Hdim ρ WFρ.
-  simpl.
-  repeat rewrite RzQ_to_base_instr_UC, instr_to_com_UC.
-  simpl; rewrite H; reflexivity.
-Qed.
-
-Lemma UC_append : forall {dim} (l1 l2: RzQ_ucom_l dim), 
-  [UC (l1 ++ l2)] =l= [UC l1] ++ [UC l2].
-Proof. 
-  intros.
-  unfold c_equiv_l, c_equiv; simpl.
-  intros.
-  repeat rewrite RzQ_to_base_instr_UC, instr_to_com_UC; simpl.
-  rewrite RzQ_to_base_ucom_l_app, list_to_ucom_append; simpl.
-  rewrite compose_super_assoc. 
-  unfold compose_super, super. Msimpl.
-  repeat rewrite Mmult_assoc.
-  reflexivity.
-Qed.
-
-Lemma UC_nil : forall dim, 
-  [UC []] =l= ([] : RzQ_com_l dim).
-Proof.
-  unfold c_equiv_l, c_equiv.
-  intros; simpl.
-  rewrite RzQ_to_base_instr_UC, instr_to_com_UC; simpl.
-  unfold compose_super, super. 
-  rewrite denote_SKIP; try assumption.
-  Msimpl; reflexivity.
-Qed.
-
-Lemma cons_to_app : forall {A} (h : A) (t : list A), h :: t = [h] ++ t.
-Proof. reflexivity. Qed.
-
-Lemma does_not_reference_c_commutes_app1 : forall {dim} (l : RzQ_com_l dim) u q,
-  does_not_reference_c l q = true ->
-  [UC [App1 u q]] ++ l =l= l ++ [UC [App1 u q]]. 
-Proof.
-  intros dim l u q H.
-  induction l using com_list_ind; try reflexivity.
-  - simpl in H.
-    apply andb_true_iff in H as [Hu0 Hl].
-    rewrite <- (app_comm_cons _ _ (UC u0)).
-    rewrite <- IHl; try assumption.
-    rewrite (cons_to_app (UC u0)).
-    rewrite (cons_to_app (UC u0) (_ ++ l)).
-    repeat rewrite app_assoc.
-    apply c_app_congruence; try reflexivity.
-    rewrite does_not_reference_instr_UC in Hu0.   
-    repeat rewrite <- UC_append.
-    apply uc_equiv_l_implies_c_equiv_l.
-    apply does_not_reference_commutes_app1.
-    assumption.
-  - simpl in H.
-    apply andb_true_iff in H as [Hmeas Hl3].
-    rewrite <- (app_comm_cons _ _ (Meas n l1 l2)).
-    rewrite <- IHl3; try assumption.
-    rewrite (cons_to_app (Meas n l1 l2)).
-    rewrite (cons_to_app (Meas n l1 l2) (_ ++ l3)).
-    repeat rewrite app_assoc.
-    apply c_app_congruence; try reflexivity.
-    rewrite does_not_reference_instr_Meas in Hmeas.
-    apply andb_true_iff in Hmeas as [Hmeas Hl2].
-    apply andb_true_iff in Hmeas as [Hq Hl1].
-    apply IHl1 in Hl1.
-    apply IHl2 in Hl2.
-    apply negb_true_iff in Hq. 
-    apply Nat.eqb_neq in Hq. 
-    clear - Hq Hl1 Hl2.
-    unfold c_equiv_l in *.
-    repeat rewrite RzQ_to_base_com_l_app, list_to_com_append in Hl1, Hl2.
-    simpl in *.
-    rewrite RzQ_to_base_instr_UC, instr_to_com_UC in *.
-    rewrite RzQ_to_base_instr_Meas, instr_to_com_Meas in *.
-    unfold c_equiv in *; simpl in *.
-    intros Hdim ρ WFρ.
-    unfold compose_super, Splus in *.
-    rewrite denote_SKIP in *; try assumption.
-    rewrite Mmult_1_l in *; try auto with wf_db.
-    remember (ueval_r dim q (RzQ_to_base u)) as U.
-    remember (pad n dim (∣1⟩ × (∣1⟩) †)) as pad1.
-    remember (pad n dim (∣0⟩ × (∣0⟩) †)) as pad0.
-    replace (super pad1 (super U ρ)) with (super U (super pad1 ρ)).
-    2: { subst; clear - Hq.
-         unfold super.
-         autorewrite with eval_db.
-         bdestruct (n + 1 <=? dim)%nat; try (Msimpl; reflexivity).
-         dependent destruction u; simpl; autorewrite with eval_db.
-         all: bdestruct (q + 1 <=? dim)%nat; try (repeat Msimpl; reflexivity).
-         all: repeat rewrite Mmult_assoc;
-              rewrite <- 2 Mmult_adjoint;
-              repeat rewrite <- Mmult_assoc.
-         all: gridify; reflexivity. } (* gridify works here too :) *)
-    replace (super pad0 (super U ρ)) with (super U (super pad0 ρ)).
-    2: { subst; clear - Hq.
-         unfold super.
-         autorewrite with eval_db.
-         bdestruct (n + 1 <=? dim)%nat; try (Msimpl; reflexivity).
-         dependent destruction u; simpl; autorewrite with eval_db.
-         all: bdestruct (q + 1 <=? dim)%nat; try (repeat Msimpl; reflexivity).
-         all: repeat rewrite Mmult_assoc;
-              rewrite <- 2 Mmult_adjoint;
-              repeat rewrite <- Mmult_assoc.
-         all: gridify; reflexivity. }
-    rewrite Hl1, Hl2; try assumption.
-    2, 3: subst; auto with wf_db.
-    unfold super. 
-    rewrite <- Mmult_plus_distr_r.
-    rewrite <- Mmult_plus_distr_l.
-    reflexivity.
-Qed.
+(* re-define for with the match_gate arg. fixed *)
+Definition remove_prefix {dim} (l pfx : RzQ_ucom_l dim) :=
+  remove_prefix l pfx (fun n => @match_gate n).
+Definition remove_suffix {dim} (l sfx : RzQ_ucom_l dim) :=
+  remove_suffix l sfx (fun n => @match_gate n).
+Definition replace_pattern {dim} (l pat rep : RzQ_ucom_l dim) :=
+  replace_pattern l pat rep (fun n => @match_gate n).
 
 (** Misc. Utilities **)
 
