VOQC/src/optimizer/GateSet.v
@@ -1,0 +1,21 @@
+Require Export UnitarySem.
+
+(* General definition of a gate set used in ListRepresentation.v.
+   An example gate set, commonly use in our optimizations, is in RzQGateSet.v. *)
+
+Module Type GateSet.
+
+  (* Gates are parameterized by a number of arguments. *)
+  Parameter U : nat -> Set.
+  
+  (* Convert U to the base_Unitary set defined in SQIR's UnitarySem.v. *)
+  Parameter to_base : forall (n : nat), U n -> base_Unitary n.
+  Arguments to_base {n}.
+
+  (* Boolean equality over gates. *)
+  Parameter match_gate : forall (n : nat), U n -> U n -> bool.
+  Arguments match_gate {n}.
+  Axiom match_gate_implies_eq : forall {n} (u u': U n), 
+    match_gate u u' = true -> to_base u = to_base u'.
+
+End GateSet.
