VOQC/benchmarks/run_voqc.sh
@@ -39,15 +39,15 @@ done
 #     python parseOutput.py ${program_name}.txt >> benchmark_results.csv
 #     rm -rf ${program_name}.txt
 # done
-# 
-# echo""
-# printf "${GREEN}##### Running on files in QFT_and_Adders #####${NOCOLOR}\n"
-# for filename in "${QFT_and_Adders_filenames[@]}"
-# do
-#     program_name=`basename "$filename" .qasm`
-#     currentTime=`date`
-#     printf "${CYAN}   + [${currentTime}] Running on ${filename}${NOCOLOR}\n"
-#     (time dune exec ./voqc.exe ${filename} out.qasm --root ../extraction) &> ${program_name}.txt
-#     python parseOutput.py ${program_name}.txt >> benchmark_results.csv
-#     rm -rf ${program_name}.txt
-# done
+
+echo""
+printf "${GREEN}##### Running on files in QFT_and_Adders #####${NOCOLOR}\n"
+for filename in "${QFT_and_Adders_filenames[@]}"
+do
+    program_name=`basename "$filename" .qasm`
+    currentTime=`date`
+    printf "${CYAN}   + [${currentTime}] Running on ${filename}${NOCOLOR}\n"
+    (time dune exec ./voqc.exe ${filename} out.qasm --root ../extraction) &> ${program_name}.txt
+    python parseOutput.py ${program_name}.txt >> benchmark_results.csv
+    rm -rf ${program_name}.txt
+done
